iodiv/IODiv.fst
@@ -427,19 +427,19 @@ let iodiv_tau #a #w (m : iodiv a w) : iodiv a w =
   assert (forall (post : wpost a). w post ==> theta (tau m) post) ;
   tau m
 
-// let twp_call #a (o : cmds) (x : io_args o) (w : io_res o -> twp a) : twp a =
+// let wcall #a (o : cmds) (x : io_args o) (w : io_res o -> twp a) : twp a =
 //   fun post -> post [] None /\ (forall y. w y (shift_post [ Call_choice o x y ] post))
 
-// let iodiv_call #a (o : cmds) (x : io_args o) #w (k : (r : io_res o) -> iodiv a (w r)) : iodiv a (twp_call o x w) =
+// let iodiv_call #a (o : cmds) (x : io_args o) #w (k : (r : io_res o) -> iodiv a (w r)) : iodiv a (wcall o x w) =
 //   call o x k
 
-// let rec twp_repeat_trunc (w : twp unit) (n : nat) : twp unit =
+// let rec wrepeat_trunc (w : twp unit) (n : nat) : twp unit =
 //   if n = 0
 //   then fun post -> True
-//   else wbind w (fun (_:unit) -> twp_tau (twp_repeat_trunc w (n - 1)))
+//   else wbind w (fun (_:unit) -> wtau (wrepeat_trunc w (n - 1)))
 
-// let twp_repeat (w : twp unit) : twp unit =
-//   fun post -> forall n. twp_repeat_trunc w n post
+// let wrepeat (w : twp unit) : twp unit =
+//   fun post -> forall n. wrepeat_trunc w n post
 
 // let repeat_unfold_1 (body : iotree unit) :
 //   Lemma (forall p. repeat body p == bind body (fun _ -> tau ((if length p = 0 then (fun _ -> loop _) else itree_cofix_unfoldn (repeat_fix body) (length p - 1)) ())) p)
@@ -500,7 +500,7 @@ let iodiv_tau #a #w (m : iodiv a w) : iodiv a w =
 //   Lemma
 //     (requires forall pp. mem pp pl ==> isRet (body pp))
 //     (ensures forall (post : wpost unit).
-//       twp_repeat_trunc w (1 + length pl) post ==>
+//       wrepeat_trunc w (1 + length pl) post ==>
 //       isEvent (body p) ==>
 //       post (ipos_trace (flatten_sep [Tau_choice] pl @ p)) None
 //     )
@@ -525,7 +525,7 @@ let iodiv_tau #a #w (m : iodiv a w) : iodiv a w =
 //   Lemma
 //     (requires forall pp. mem pp pl ==> isRet (body pp))
 //     (ensures forall (post : wpost unit).
-//       twp_repeat_trunc w (1 + length pl) post ==>
+//       wrepeat_trunc w (1 + length pl) post ==>
 //       isRet (body p) ==>
 //       post (ipos_trace (flatten_sep [Tau_choice] pl @ p)) None
 //     )
@@ -533,19 +533,19 @@ let iodiv_tau #a #w (m : iodiv a w) : iodiv a w =
 // = match pl with
 //   | [] ->
 //     assert (forall (post : wpost unit).
-//       twp_repeat_trunc w 1 post ==>
+//       wrepeat_trunc w 1 post ==>
 //       isRet (body p) ==>
-//       twp_tau (twp_repeat_trunc w 0) (shift_post (ipos_trace p) post)
+//       wtau (wrepeat_trunc w 0) (shift_post (ipos_trace p) post)
 //     )
 //   | pp :: pl ->
 //     repeat_any_ret_ret_post body pl p ;
 //     assert (forall (post : wpost unit).
-//       twp_repeat_trunc w (1 + length pl) post ==>
+//       wrepeat_trunc w (1 + length pl) post ==>
 //       isRet (body p) ==>
 //       post (ipos_trace (flatten_sep [Tau_choice] pl @ p)) None
 //     ) ;
 //     assert (forall (post : wpost unit).
-//       twp_repeat_trunc w (1 + length pl) (shift_post (ipos_trace pp) post) ==>
+//       wrepeat_trunc w (1 + length pl) (shift_post (ipos_trace pp) post) ==>
 //       isRet (body p) ==>
 //       shift_post (ipos_trace pp) post (ipos_trace (flatten_sep [Tau_choice] pl @ p)) None
 //     ) ;
@@ -561,12 +561,12 @@ let iodiv_tau #a #w (m : iodiv a w) : iodiv a w =
 //       ipos_trace pp @ ipos_trace (flatten_sep [Tau_choice] pl @ p) ;
 //     } ;
 //     assert (forall (post : wpost unit).
-//       twp_repeat_trunc w (1 + length pl) (shift_post (ipos_trace pp) post) ==>
+//       wrepeat_trunc w (1 + length pl) (shift_post (ipos_trace pp) post) ==>
 //       isRet (body p) ==>
 //       post (ipos_trace (flatten_sep [Tau_choice] (pp :: pl) @ p)) None
 //     ) ;
 //     assert (forall (post : wpost unit).
-//       twp_repeat_trunc w (2 + length pl) post ==>
+//       wrepeat_trunc w (2 + length pl) post ==>
 //       isRet (body p) ==>
 //       post (ipos_trace (flatten_sep [Tau_choice] (pp :: pl) @ p)) None
 //     )
@@ -575,7 +575,7 @@ let iodiv_tau #a #w (m : iodiv a w) : iodiv a w =
 //   Lemma
 //     (requires forall pp. mem pp pl ==> isRet (body pp))
 //     (ensures forall (post : wpost unit).
-//       twp_repeat w post ==>
+//       wrepeat w post ==>
 //       isEvent (repeat body (flatten_sep [Tau_choice] pl @ p)) ==>
 //       post (ipos_trace (flatten_sep [Tau_choice] pl @ p)) None
 //     )
@@ -592,9 +592,9 @@ let iodiv_tau #a #w (m : iodiv a w) : iodiv a w =
 //       assert (repeat body p == Some Tau) ;
 //       repeat_any_ret_ret_post body pl p ;
 //       assert (isRet (body p)) ;
-//       assert (forall (post : wpost unit). twp_repeat w post ==> twp_repeat_trunc w (1 + length pl) post) ;
+//       assert (forall (post : wpost unit). wrepeat w post ==> wrepeat_trunc w (1 + length pl) post) ;
 //       assert (forall (post : wpost unit).
-//         twp_repeat w post ==>
+//         wrepeat w post ==>
 //         isEvent (repeat body p) ==>
 //         post (ipos_trace (flatten_sep [Tau_choice] pl @ p)) None
 //       )
@@ -615,26 +615,26 @@ let iodiv_tau #a #w (m : iodiv a w) : iodiv a w =
 //   | None ->
 //     repeat_any_ret body pl p ;
 //     repeat_any_ret_event_post body pl p ;
-//     assert (forall (post : wpost unit). twp_repeat w post ==> twp_repeat_trunc w (1 + length pl) post) ;
+//     assert (forall (post : wpost unit). wrepeat w post ==> wrepeat_trunc w (1 + length pl) post) ;
 //     repeat_unfold_1 body ;
 //     assert (
 //       isEvent (repeat body p) ==> isEvent (body p)
 //     ) ;
 //     assert (forall (post : wpost unit).
-//       twp_repeat w post ==>
+//       wrepeat w post ==>
 //       isEvent (repeat body p) ==>
 //       post (ipos_trace (flatten_sep [Tau_choice] pl @ p)) None
 //     )
 
 // let iodiv_repeat_proof #w (body : iodiv unit w) p :
 //   Lemma (forall (post : wpost unit).
-//     twp_repeat w post ==>
+//     wrepeat w post ==>
 //     isEvent (repeat body p) ==>
 //     post (ipos_trace p) None
 //   )
 // = iodiv_repeat_proof_gen body [] p
 
-// let iodiv_repeat #w (body : iodiv unit w) : iodiv unit (twp_repeat w) =
+// let iodiv_repeat #w (body : iodiv unit w) : iodiv unit (wrepeat w) =
 //   forall_intro (repeat_not_ret body) ;
 //   forall_intro (iodiv_repeat_proof body) ;
 //   repeat body
@@ -654,42 +654,42 @@ let iodiv_tau #a #w (m : iodiv a w) : iodiv a w =
 //   inv [] /\
 //   (forall tr. inv tr ==> w (fun tr' v -> inv (tr @ tr') /\ Some? v))
 
-// let twp_repeat_with_inv (w : twp unit) (inv : trace -> Type0) : twp unit =
+// let wrepeat_with_inv (w : twp unit) (inv : trace -> Type0) : twp unit =
 //   fun post -> forall tr. inv tr ==> post tr None
 
 // let invpost (inv : trace -> Type0) : wpost unit =
 //   fun tr v -> inv tr /\ None? v
 
 // // Maybe prove it on the effect observation directly
-// let rec twp_repeat_inv_trunc (w : twp unit) (inv : trace -> Type0) n :
+// let rec wrepeat_inv_trunc (w : twp unit) (inv : trace -> Type0) n :
 //   Lemma (
 //     trace_invariant w inv ==>
-//     twp_repeat_trunc w n (invpost inv)
+//     wrepeat_trunc w n (invpost inv)
 //   )
 // = if n = 0
 //   then ()
 //   else begin
-//     twp_repeat_inv_trunc w inv (n - 1) ;
+//     wrepeat_inv_trunc w inv (n - 1) ;
 //     assume (
 //       trace_invariant w inv ==>
-//       twp_repeat_trunc w (n-1) (invpost inv) ==>
-//       wbind w (fun (_:unit) -> twp_tau (twp_repeat_trunc w (n - 1))) (invpost inv)
+//       wrepeat_trunc w (n-1) (invpost inv) ==>
+//       wbind w (fun (_:unit) -> wtau (wrepeat_trunc w (n - 1))) (invpost inv)
 //       // ==
 //       // w (fun tr v ->
 //       //   match v with
-//       //   | Some x -> (fun (_:unit) -> twp_tau (twp_repeat_trunc w (n - 1))) x (shift_post tr (invpost inv))
-//       //     == twp_tau (twp_repeat_trunc w (n - 1)) (shift_post tr (invpost inv))
+//       //   | Some x -> (fun (_:unit) -> wtau (wrepeat_trunc w (n - 1))) x (shift_post tr (invpost inv))
+//       //     == wtau (wrepeat_trunc w (n - 1)) (shift_post tr (invpost inv))
 //       //   | None -> invpost inv tr None // == inv tr
 //       // )
 //     ) ;
 //     assume (forall (post : wpost unit).
-//       wbind w (fun (_:unit) -> twp_tau (twp_repeat_trunc w (n - 1))) post ==>
-//       twp_repeat_trunc w n post
+//       wbind w (fun (_:unit) -> wtau (wrepeat_trunc w (n - 1))) post ==>
+//       wrepeat_trunc w n post
 //     ) ; // why??
 //     assert (
 //       trace_invariant w inv ==>
-//       twp_repeat_trunc w (n-1) (invpost inv) ==>
-//       twp_repeat_trunc w n (invpost inv)
+//       wrepeat_trunc w (n-1) (invpost inv) ==>
+//       wrepeat_trunc w n (invpost inv)
 //     )
 //   end
 
@@ -705,33 +705,33 @@ let iodiv_tau #a #w (m : iodiv a w) : iodiv a w =
 // // let ret_terminates a (x : a) : Lemma (wret x terminates) = ()
 
 // // Should be p1 ==> p2 rather than ==
-// let rec twp_repeat_trunc_ext w n (p1 p2 : wpost unit) :
-//   Lemma ((forall tr x. p1 tr x == p2 tr x) ==> twp_repeat_trunc w n p1 == twp_repeat_trunc w n p2)
+// let rec wrepeat_trunc_ext w n (p1 p2 : wpost unit) :
+//   Lemma ((forall tr x. p1 tr x == p2 tr x) ==> wrepeat_trunc w n p1 == wrepeat_trunc w n p2)
 // = if n = 0
 //   then ()
 //   else begin
-//     // twp_repeat_trunc_ext w (n-1) p1 p2 ;
-//     // assume ((forall tr x. p1 tr x == p2 tr x) ==> wbind w (fun _ -> twp_repeat_trunc w (n -1)) p1 == wbind w (fun _ -> twp_repeat_trunc w (n -1)) p2)
-//     // assert (twp_repeat_trunc w n == wbind w (fun _ -> twp_repeat_trunc w (n -1))) ; // Isn't this by def??
-//     assume ((forall tr x. p1 tr x == p2 tr x) ==> twp_repeat_trunc w n p1 == twp_repeat_trunc w n p2)
+//     // wrepeat_trunc_ext w (n-1) p1 p2 ;
+//     // assume ((forall tr x. p1 tr x == p2 tr x) ==> wbind w (fun _ -> wrepeat_trunc w (n -1)) p1 == wbind w (fun _ -> wrepeat_trunc w (n -1)) p2)
+//     // assert (wrepeat_trunc w n == wbind w (fun _ -> wrepeat_trunc w (n -1))) ; // Isn't this by def??
+//     assume ((forall tr x. p1 tr x == p2 tr x) ==> wrepeat_trunc w n p1 == wrepeat_trunc w n p2)
 //   end
 
 // let repeat_ret_loops () :
-//   Lemma (twp_repeat (wret ()) diverges)
+//   Lemma (wrepeat (wret ()) diverges)
 // = let rec aux n :
-//     Lemma (twp_repeat_trunc (wret ()) n diverges) [SMTPat ()]
+//     Lemma (wrepeat_trunc (wret ()) n diverges) [SMTPat ()]
 //   = if n = 0
 //     then ()
 //     else begin
 //       aux (n - 1) ;
-//       twp_repeat_trunc_ext (wret ()) (n-1) (shift_post [] diverges) (diverges #unit)
+//       wrepeat_trunc_ext (wret ()) (n-1) (shift_post [] diverges) (diverges #unit)
 //     end
 //   in
 //   ()
 
 // // Much better
 // let repeat_ret_loops_with_inv () :
-//   Lemma (twp_repeat_with_inv (wret ()) (fun _ -> True) diverges)
+//   Lemma (wrepeat_with_inv (wret ()) (fun _ -> True) diverges)
 // = ()
 
 // [@@allow_informative_binders]
